Small changes

Common.fst
@@ -4,6 +4,18 @@ open FStar.Exn
 
 type maybe a = either a exn
 
+let compose g f = fun x -> g (f x)
+
+let id #a (x:a) = x
+
+unfold let inl_app #a #b (f:a -> b) (x:maybe a) : maybe b =
+  match x with
+  | Inl x -> Inl (f x)
+  | Inr err -> Inr err
+
+  
+let cdr #a (_, (x:a)) : a = x
+
 let elim_pure #a #wp ($f : unit -> PURE a wp) p
  : Pure a (requires (wp p)) (ensures (fun r -> p r))
  //: PURE a (fun p' -> wp p /\ (forall r. p r ==> p' r))
